Prove all_extract_bytes_from_uvalue_strict_subterm.
- Remove extraneous definition of all_extract_bytes_from_uvalue.

src/coq/Handlers/Concretization.v
@@ -322,8 +322,6 @@ Module Type ConcretizationBase (LP : LLVMParams) (MP : MemoryParams LP) (Byte : 
     forall (M : Type -> Type) `{Monad M} (handler : dtyp -> M dvalue) (ERR_M : Type -> Type) `{Monad ERR_M} `{RAISE_ERROR ERR_M} `{RAISE_UB ERR_M} `{RAISE_OOM ERR_M},
       (forall A : Type, ERR_M A -> M A) -> list uvalue -> dtyp -> M dvalue.
 
-  Parameter all_extract_bytes_from_uvalue : dtyp -> list uvalue -> option uvalue.
-
   Parameter eval_select :
     forall (M : Type -> Type) `{Monad M} (handler : dtyp -> M dvalue)
       (ERR_M : Type -> Type) `{Monad ERR_M} `{RAISE_ERROR ERR_M} `{RAISE_UB ERR_M} `{RAISE_OOM ERR_M}
@@ -417,7 +415,7 @@ Module Type ConcretizationBase (LP : LLVMParams) (MP : MemoryParams LP) (Byte : 
         | UVALUE_ConcatBytes bytes dt =>
             if N.of_nat (Datatypes.length bytes) =? sizeof_dtyp dt
             then
-              match all_extract_bytes_from_uvalue dt bytes with
+              match Byte.all_extract_bytes_from_uvalue dt bytes with
               | Some uv => concretize_uvalueM M undef_handler ERR_M lift_ue uv
               | None => extractbytes_to_dvalue M undef_handler ERR_M lift_ue bytes dt
               end
@@ -943,29 +941,6 @@ Module MakeBase (LP : LLVMParams) (MP : MemoryParams LP) (Byte : ByteModule LP.A
 
   Definition endianess : Endianess
     := ENDIAN_LITTLE.
-
-  Fixpoint all_extract_bytes_from_uvalue_helper (idx' : N) (sid' : store_id) (dt' : dtyp) (parent : uvalue) (bytes : list uvalue) : option uvalue
-    := match bytes with
-       | [] => Some parent
-       | (UVALUE_ExtractByte uv dt idx sid)::bytes =>
-           guard_opt (N.eqb idx idx');;
-           guard_opt (RelDec.rel_dec uv parent);;
-           guard_opt (N.eqb sid sid');;
-           guard_opt (dtyp_eqb dt dt');;
-           all_extract_bytes_from_uvalue_helper (N.succ idx') sid' dt' parent bytes
-       | _ => None
-       end.
-
-  (* Check that store ids, uvalues, and types match up, as well as
-       that the extract byte indices are in the right order *)
-  Definition all_extract_bytes_from_uvalue (t : dtyp) (bytes : list uvalue) : option uvalue
-    := match bytes with
-       | nil => None
-       | (UVALUE_ExtractByte uv dt idx sid)::xs =>
-           guard_opt (dtyp_eqb t dt);;
-           all_extract_bytes_from_uvalue_helper 0 sid dt uv bytes
-       | _ => None
-       end.
 
   (* Definition fp_alignment (bits : N) : option Alignment := *)
   (*   let fp_map := dl_floating_point_alignments datalayout *)
